scripts/gooseall.sh
@@ -14,6 +14,7 @@ scripts/goose.sh -dir kubernetes ./staging/src/k8s.io/api/core/v1
 scripts/goose.sh -dir kubernetes ./staging/src/k8s.io/api/apps/v1
 scripts/goose.sh -dir kubernetes ./staging/src/k8s.io/apimachinery/pkg/api/errors
 scripts/goose.sh -dir kubernetes ./staging/src/k8s.io/apimachinery/pkg/api/meta
+scripts/goose.sh -dir kubernetes ./staging/src/k8s.io/apimachinery/pkg/api/resource
 scripts/goose.sh -dir kubernetes ./staging/src/k8s.io/apimachinery/pkg/apis/meta/v1
 scripts/goose.sh -dir kubernetes ./staging/src/k8s.io/apimachinery/pkg/labels
 scripts/goose.sh -dir kubernetes ./staging/src/k8s.io/apimachinery/pkg/runtime/schema
